wip

Logic/Modal/Standard/Kripke/Completeness.lean
@@ -6,14 +6,54 @@ namespace LO.System
 
 variable {F : Type*} [LogicalConnective F] [DecidableEq F]
 variable {S : Type*} [System F S]
-variable {𝓢 : S}
-variable [Minimal 𝓢]
+variable {𝓢 : S} {p q r : F} {Γ Δ : List F} {T : Set F}
+variable [Minimal 𝓢] [NegDefinition F]
 
-lemma dhyp! (q : F) (b : 𝓢 ⊢! p) : 𝓢 ⊢! q ⟶ p := ⟨dhyp q b.some⟩
+open FiniteContext
+
+lemma FiniteContext.of'! (h : 𝓢 ⊢! p) : Γ ⊢[𝓢]! p := weakening! (by simp) $ provable_iff_provable.mp h
+lemma FiniteContext.toₛ! (b : Γ ⊢[𝓢]! p) : 𝓢 ⊢! Γ.conj ⟶ p := b
+
+lemma implyLeft_conj_eq_conj' : 𝓢 ⊢! Γ.conj ⟶ p ↔ 𝓢 ⊢! Γ.conj' ⟶ p := implyLeftReplaceIff'! (by
+  induction Γ using List.induction_with_singleton with
+  | hnil => simp;
+  | hsingle q =>
+    simp;
+    apply iff_intro! (by simp) (by
+      apply provable_iff_provable.mpr;
+      apply deduct_iff.mpr;
+      exact conj₃'! (by_axm! (by simp)) (by simp)
+    );
+  | hcons q Γ hΓ ih =>
+    simp [(List.conj'_cons_nonempty (a := q) hΓ)];
+    apply iff_intro!
+      (by
+        apply provable_iff_provable.mpr;
+        apply deduct_iff.mpr;
+        have d : [q ⋏ List.conj Γ] ⊢[𝓢]! q ⋏ List.conj Γ := by_axm! (by simp);
+        exact conj₃'! (conj₁'! d) ((of'! $ conj₁'! ih) ⨀ (conj₂'! d))
+      )
+      (by
+        apply provable_iff_provable.mpr;
+        apply deduct_iff.mpr;
+        have d : [q ⋏ List.conj' Γ] ⊢[𝓢]! q ⋏ List.conj' Γ := by_axm! (by simp);
+        exact conj₃'! (conj₁'! d) ((of'! $ conj₂'! ih) ⨀ (conj₂'! d))
+      )
+  )
+
+@[simp]
+lemma dn_iff! [NegDefinition F] [HasDNE 𝓢] : 𝓢 ⊢! p ⟷ ~~p := iff_intro! (by simp) (by simp)
+
+lemma supplemental1 [NegDefinition F] [HasEFQ 𝓢] (h : 𝓢 ⊢! ~p) : 𝓢 ⊢! p ⟶ q := by
+  apply provable_iff_provable.mpr;
+  apply deduct_iff.mpr;
+  have dnp : [p] ⊢[𝓢]! p ⟶ ⊥ := by simpa [NegDefinition.neg] using of'! h;
+  have dp : [p] ⊢[𝓢]! p := by_axm! (by simp);
+  exact efq'! (dnp ⨀ dp);
 
 namespace Context
 
-lemma by_axm! {p} (h : p ∈ Γ) : Γ *⊢[𝓢]! p := by
+lemma by_axm! {p} (h : p ∈ T) : T *⊢[𝓢]! p := by
   apply provable_iff.mpr;
   existsi {p};
   constructor;
@@ -30,42 +70,55 @@ namespace LO.Modal.Standard
 variable [DecidableEq α]
 
 @[simp]
-def Theory.ΛConsistent (Λ : AxiomSet α) (T : Theory α) := ∀ Γ : List (Formula α), (∀ p ∈ Γ, p ∈ T) → Λ ⊬! Γ.conj ⟶ ⊥
+def Theory.ΛConsistent (Λ : AxiomSet α) (T : Theory α) := ∀ {Γ : List (Formula α)}, (∀ p ∈ Γ, p ∈ T) → Λ ⊬! Γ.conj' ⟶ ⊥
 notation:max "(" Λ ")-Consistent " T:90 => Theory.ΛConsistent Λ T
 
 variable {Λ : AxiomSet α}
-variable {T : Theory α} (consisT : (Λ)-Consistent T)
 
 open System
 open Theory
 
 namespace Theory
 
-variable (consisT : (Λ)-Consistent T)
+variable {T : Theory α} (consisT : (Λ)-Consistent T)
+
+lemma unprovable_either : ¬(T *⊢[Λ]! p ∧ T *⊢[Λ]! ~p) := by
+  by_contra hC;
+  have ⟨hC₁, hC₂⟩ := hC;
+  have : T *⊢[Λ]! ⊥ := hC₂ ⨀ hC₁;
+  obtain ⟨Γ, hΓ₁, hΓ₂⟩ := Context.provable_iff.mp this;
+  have : Λ ⊬! List.conj' Γ ⟶ ⊥ := consisT hΓ₁;
+  have : Λ ⊢! List.conj' Γ ⟶ ⊥ := implyLeft_conj_eq_conj'.mp $ FiniteContext.toₛ! hΓ₂;
+  contradiction;
+
+
+lemma provable_iff_insert_neg_not_Λconsistent : T *⊢[Λ]! p ↔ ¬(Λ)-Consistent (insert (~p) T) := by sorry;
+
+lemma neg_provable_iff_insert_not_Λconsistent : T *⊢[Λ]! ~p ↔ ¬(Λ)-Consistent (insert (p) T) := by sorry;
+
 
 lemma not_provable_falsum : Λ ⊬! ⊥ := by
   by_contra hC;
-  have : Λ ⊢! ⊤ ⟶ ⊥ := dhyp! ⊤ hC;
-  have : Λ ⊬! ⊤ ⟶ ⊥ := by simpa [Finset.conj] using consisT ∅ (by simp);
+  have : Λ ⊢! ⊤ ⟶ ⊥ := dhyp! hC;
+  have : Λ ⊬! ⊤ ⟶ ⊥ := by simpa [Finset.conj] using consisT (Γ := []) (by simp);
   contradiction;
 
 lemma not_mem_falsum_of_Λconsistent : ⊥ ∉ T := by
   by_contra hC;
-  have : Λ ⊬! ⊥ ⟶ ⊥ := implyLeftConjSingleton!.not.mp $ consisT _ (by simpa);
+  have : Λ ⊬! ⊥ ⟶ ⊥ := consisT (Γ := [⊥]) (by simpa);
   have : Λ ⊢! ⊥ ⟶ ⊥ := efq!;
   contradiction;
 
-end Theory
-
-lemma exists_maximal_consistent_theory :
-  ∃ Z, (Λ)-Consistent Z ∧ T ⊆ Z ∧ ∀ U, (Λ)-Consistent U → Z ⊆ U → U = Z
+lemma exists_maximal_Λconsistent_theory
+  : ∃ Z, (Λ)-Consistent Z ∧ T ⊆ Z ∧ ∀ U, (Λ)-Consistent U → Z ⊆ U → U = Z
   := zorn_subset_nonempty { T : Theory α | (Λ)-Consistent T } (by
     intro c hc chain hnc;
     existsi (⋃₀ c);
     simp only [ΛConsistent, Set.mem_setOf_eq, Set.mem_sUnion];
     constructor;
-    . by_contra hC;
-      obtain ⟨Γ, hΓs, hΓd⟩ := by simpa using hC;
+    . intro Γ;
+      by_contra hC;
+      obtain ⟨hΓs, hΓd⟩ := by simpa using hC;
       obtain ⟨U, hUc, hUs⟩ :=
         Set.subset_mem_chain_of_finite c hnc chain
           (s := ↑Γ.toFinset) (by simp)
@@ -83,6 +136,8 @@ lemma exists_maximal_consistent_theory :
       exact Set.subset_sUnion_of_mem a;
   ) T consisT
 
+end Theory
+
 structure MaximalConsistentByTheory (Λ : AxiomSet α) where
   theory : Theory α
   consistent : (Λ)-Consistent theory
@@ -95,39 +150,8 @@ namespace MaximalConsistentByTheory
 variable {Ω Ω₁ Ω₂ : MCT Λ}
 variable {p : Formula α}
 
-@[simp]
-lemma unprovable_falsum : Ω.theory *⊬[Λ]! ⊥ := by
-  have := Theory.not_provable_falsum Ω.consistent;
-  by_contra hC;
-  have := Context.provable_iff.mp hC;
-  sorry;
-
-lemma membership_iff : (p ∈ Ω.theory) ↔ (Ω.theory *⊢[Λ]! p) := by
-  constructor;
-  . intro h; exact Context.by_axm! h;
-  . intro hp;
-    suffices ~p ∉ Ω.theory by sorry;
-    by_contra hC;
-    have hnp : Ω.theory *⊢[Λ]! ~p := Context.by_axm! hC;
-    have : Ω.theory *⊢[Λ]! ⊥ := hnp ⨀ hp;
-    have : Ω.theory *⊬[Λ]! ⊥ := unprovable_falsum;
-    contradiction;
-
-lemma iff_congr : (Ω.theory *⊢[Λ]! (p ⟷ q)) → ((p ∈ Ω.theory) ↔ (q ∈ Ω.theory)) := by
-  simp only [LogicalConnective.iff];
-  intro hpq;
-  constructor;
-  . intro hp;
-    exact membership_iff.mpr $ (conj₁'! hpq) ⨀ (membership_iff.mp hp)
-  . intro hq;
-    exact membership_iff.mpr $ (conj₂'! hpq) ⨀ (membership_iff.mp hq)
-
-lemma mem_dn_iff : (p ∈ Ω.theory) ↔ (~~p ∈ Ω.theory) := iff_congr $ (by sorry)
-
-end MaximalConsistentByTheory
-
-lemma exists_maximal_consistented_theory : ∃ (Ω : MCT Λ), (T ⊆ Ω.theory) := by
-  have ⟨Ω, hΩ₁, hΩ₂, hΩ₃⟩ := exists_maximal_consistent_theory consisT;
+lemma exists_maximal_Λconsistented_theory (consisT : (Λ)-Consistent T) : ∃ (Ω : MCT Λ), (T ⊆ Ω.theory) := by
+  have ⟨Ω, hΩ₁, hΩ₂, hΩ₃⟩ := exists_maximal_Λconsistent_theory consisT;
   existsi ⟨
     Ω,
     hΩ₁,
@@ -140,9 +164,128 @@ lemma exists_maximal_consistented_theory : ∃ (Ω : MCT Λ), (T ⊆ Ω.theory) 
   ⟩;
   simp_all only [ΛConsistent];
 
-alias lindenbaum := exists_maximal_consistented_theory
+alias lindenbaum := exists_maximal_Λconsistented_theory
+
+lemma maximal' {p : Formula α} (hp : p ∉ Ω.theory) : ¬(Λ)-Consistent (insert p Ω.theory) := Ω.maximal (Set.ssubset_insert hp)
+
+
+lemma membership_iff : (p ∈ Ω.theory) ↔ (Ω.theory *⊢[Λ]! p) := by
+  constructor;
+  . intro h;
+    exact Context.by_axm! h;
+  . intro hp;
+    by_contra hC;
+
+    obtain ⟨Γ, hΓ₁, hΓ₂⟩ := hp;
+    obtain ⟨Δ, hΔ₁, hΔ₂⟩ := neg_provable_iff_insert_not_Λconsistent.mpr $ Ω.maximal (Set.ssubset_insert hC);
+
+    replace hΓ₂ : (Γ ++ Δ) ⊢[Λ]! p := FiniteContext.weakening! (by simp) ⟨hΓ₂⟩
+    replace hΔ₂ : (Γ ++ Δ) ⊢[Λ]! ~p := FiniteContext.weakening! (by simp) ⟨hΔ₂⟩
+
+    have : Λ ⊢! List.conj' (Γ ++ Δ) ⟶ ⊥ := implyLeft_conj_eq_conj'.mp $ FiniteContext.provable_iff.mp (hΔ₂ ⨀ hΓ₂);
+    have : Λ ⊬! List.conj' (Γ ++ Δ) ⟶ ⊥ := Ω.consistent (by simp; rintro q (hq₁ | hq₂); exact hΓ₁ _ hq₁; exact hΔ₁ _ hq₂);
+    contradiction;
+
+@[simp]
+lemma not_mem_falsum : ⊥ ∉ Ω.theory := not_mem_falsum_of_Λconsistent Ω.consistent
+
+@[simp]
+lemma unprovable_falsum : Ω.theory *⊬[Λ]! ⊥ := by apply membership_iff.not.mp; simp
+
+lemma iff_mem_neg : (~p ∈ Ω.theory) ↔ (p ∉ Ω.theory) := by
+  constructor;
+  . intro hnp;
+    by_contra hp;
+    replace hp := membership_iff.mp hp;
+    replace hnp := membership_iff.mp hnp;
+    have : Ω.theory *⊢[Λ]! ⊥ := hnp ⨀ hp;
+    have : Ω.theory *⊬[Λ]! ⊥ := unprovable_falsum;
+    contradiction;
+  . intro hp;
+    have := provable_iff_insert_neg_not_Λconsistent.not.mp $ membership_iff.not.mp hp;
+    have := (not_imp_not.mpr $ Ω.maximal (U := insert (~p) Ω.theory)) this;
+    simp [Set.ssubset_def] at this;
+    apply this;
+    simp;
+
+@[simp]
+lemma iff_mem_imp : ((p ⟶ q) ∈ Ω.theory) ↔ (p ∈ Ω.theory) → (q ∈ Ω.theory) := by
+  constructor;
+  . intro hpq hp;
+    replace dpq := membership_iff.mp hpq;
+    replace dp  := membership_iff.mp hp;
+    apply membership_iff.mpr;
+    exact dpq ⨀ dp;
+  . intro h;
+    replace h : p ∉ Ω.theory ∨ q ∈ Ω.theory := or_iff_not_imp_left.mpr (by simpa using h);
+    cases h with
+    | inl h =>
+      apply membership_iff.mpr;
+      exact supplemental1 $ membership_iff.mp $ iff_mem_neg.mpr h;
+    | inr h =>
+      apply membership_iff.mpr;
+      exact imply₁! ⨀ (membership_iff.mp h)
+
+@[simp]
+lemma iff_mem_and : ((p ⋏ q) ∈ Ω.theory) ↔ (p ∈ Ω.theory) ∧ (q ∈ Ω.theory) := by
+  constructor;
+  . intro hpq;
+    replace hpq := membership_iff.mp hpq;
+    constructor;
+    . apply membership_iff.mpr; exact conj₁'! hpq;
+    . apply membership_iff.mpr; exact conj₂'! hpq;
+  . rintro ⟨hp, hq⟩;
+    apply membership_iff.mpr;
+    exact conj₃'! (membership_iff.mp hp) (membership_iff.mp hq);
+
+@[simp]
+lemma iff_mem_or : ((p ⋎ q) ∈ Ω.theory) ↔ (p ∈ Ω.theory) ∨ (q ∈ Ω.theory) := by
+  constructor;
+  . intro hpq;
+    replace hpq := membership_iff.mp hpq;
+    by_contra hC; simp [not_or] at hC;
+    have ⟨hp, hq⟩ := hC;
+    replace hp := membership_iff.mp $ iff_mem_neg.mpr hp;
+    replace hq := membership_iff.mp $ iff_mem_neg.mpr hq;
+    have : Ω.theory *⊢[Λ]! ⊥ := disj₃'! hp hq hpq;
+    have : Ω.theory *⊬[Λ]! ⊥ := unprovable_falsum;
+    contradiction;
+  . rintro (hp | hq);
+    . apply membership_iff.mpr;
+      exact disj₁'! (membership_iff.mp hp);
+    . apply membership_iff.mpr;
+      exact disj₂'! (membership_iff.mp hq);
+
+lemma iff_mem_box : (□p ∈ Ω.theory) ↔ (∀ {Ω' : MCT Λ}, (□⁻¹Ω.theory ⊆ Ω'.theory) → (p ∈ Ω'.theory)) := by
+  constructor;
+  . intro hp Ω' hΩ'
+    apply hΩ';
+    simpa;
+  . contrapose;
+    intro hp;
+    have : (Λ)-Consistent (insert (~p) (□⁻¹Ω.theory)) := by sorry;
+    obtain ⟨Ω', hΩ'⟩ := lindenbaum this;
+    push_neg;
+    existsi Ω';
+    constructor;
+    . exact Set.Subset.trans (by simp_all) hΩ';
+    . apply iff_mem_neg.mp;
+      apply hΩ';
+      simp only [Set.mem_insert_iff, true_or]
+
+lemma iff_congr : (Ω.theory *⊢[Λ]! (p ⟷ q)) → ((p ∈ Ω.theory) ↔ (q ∈ Ω.theory)) := by
+  intro hpq;
+  constructor;
+  . intro hp; exact iff_mem_imp.mp (membership_iff.mpr $ conj₁'! hpq) hp;
+  . intro hq; exact iff_mem_imp.mp (membership_iff.mpr $ conj₂'! hpq) hq;
+
+lemma mem_dn_iff : (p ∈ Ω.theory) ↔ (~~p ∈ Ω.theory) := iff_congr $ (by simp)
+
+end MaximalConsistentByTheory
+
 
 open Formula
+open MaximalConsistentByTheory
 
 namespace Kripke
 
@@ -150,8 +293,11 @@ def CanonicalModel (Λ : AxiomSet α) : Model (MCT Λ) α where
   frame (Ω₁ Ω₂) := □⁻¹Ω₁.theory ⊆ Ω₂.theory
   valuation Ω a := (atom a) ∈ Ω.theory
 
+abbrev CanonicalFrame (Λ : AxiomSet α) : Frame (MCT Λ) α := CanonicalModel Λ |>.frame
+
 namespace CanonicalModel
 
+@[simp]
 lemma frame_def: (CanonicalModel Λ).frame Ω₁ Ω₂ ↔ (∀ {p : Formula α}, □p ∈ Ω₁.theory → p ∈ Ω₂.theory) := by rfl
 
 @[simp]
@@ -159,29 +305,52 @@ lemma val_def {a : α} : (CanonicalModel Λ).valuation Ω a ↔ (atom a) ∈ Ω.
 
 end CanonicalModel
 
-lemma truthlemma {p : Formula α} : ∀ {Ω : MCT Λ}, ((CanonicalModel Λ, Ω) ⊧ p) ↔ (p ∈ Ω.theory) := by
-  sorry;
-  /-
+lemma truthlemma {p : Formula α} : ∀ {Ω : MCT Λ}, (CanonicalModel Λ, Ω) ⊧ p ↔ (p ∈ Ω.theory) := by
   induction p using Formula.rec' with
-  | hatom => simp;
-  | hfalsum => simp;
-  | himp => simp_all [imp_membership_iff'];
-  | hor => simp_all [or_membership_iff];
-  | hand => simp_all [and_membership_iff];
   | hbox p ih =>
     intro Ω;
     constructor;
     . intro h;
-      apply (mct_mem_box_iff hK).mpr;
+      apply iff_mem_box.mpr;
       intro Ω' hΩ';
       apply ih.mp;
-      simp [Satisfies.box_def] at h;
       exact h Ω' hΩ';
     . intro h Ω' hΩ';
       apply ih.mpr;
       simp [Set.subset_def, CanonicalModel.frame_def] at hΩ';
       exact hΩ' h;
-  -/
+  | _ => simp_all
+
+lemma deducible_of_validOnCanonicelModel : (CanonicalModel Λ) ⊧ p → (Λ ⊢! p) := by
+  contrapose;
+  intro h;
+  have : (Λ)-Consistent ({~p}) := by sorry;
+  obtain ⟨Ω, hΩ⟩ := lindenbaum this;
+  simp [Kripke.ValidOnModel];
+  existsi Ω;
+  exact truthlemma.not.mpr $ iff_mem_neg.mp (show ~p ∈ Ω.theory by simp_all);
+
+class Canonical (Λ : AxiomSet α) where
+  property : Frame (MCT Λ) α → Prop
+  definability : AxiomSetDefinability (MCT Λ) Λ property
+  satisfy : property (CanonicalFrame Λ)
+
+lemma complete!_of_canonically [c : Canonical Λ] : 𝔽((Λ : AxiomSet α), MCT (Λ : AxiomSet α)) ⊧ p → (Λ ⊢! p) := by
+  contrapose;
+  intro h₁ h₂;
+  simp [Kripke.ValidOnFrameClass, Kripke.ValidOnFrame] at h₂;
+  have : Λ ⊢! p := deducible_of_validOnCanonicelModel $ h₂ (CanonicalModel Λ).frame
+    (by apply iff_definability_memAxiomSetFrameClass c.definability |>.mp; exact c.satisfy)
+    (CanonicalModel Λ).valuation;
+  contradiction;
+
+instance [Canonical Λ] : Complete (Λ : AxiomSet α) 𝔽(Λ, MCT Λ) := ⟨complete!_of_canonically⟩
+
+instance : Canonical (𝐊 : AxiomSet α) where
+  definability := AxiomSet.K.definability
+  satisfy := by simp;
+
+instance : Complete (𝐊 : AxiomSet α) 𝔽((𝐊 : AxiomSet α), MCT (𝐊 : AxiomSet α)) := inferInstance
 
 end Kripke
 
